Revert "An attempt at separating idiom notation from pure"
This reverts commit cca999df4b4330261944bc5634fc665d8aa8c87a.

MPL/SPred/SVal.lean
@@ -20,42 +20,6 @@ def pure {σs : List Type} (a : α) : SVal σs α := match σs with
 @[simp] theorem pure_nil (a : α) : pure (σs:=[]) a = a := rfl
 @[simp] theorem pure_cons {s : σ} (a : α) : pure (σs:=σ::σs) a s = pure a := rfl
 
-/-- Pack all state variables into a tuple.
-This type will be looked up `by assumption` to implement idiom notation. -/
-def StateTuple (σs : List Type) := match σs with
-| [] => Unit
-| σ :: σs => σ × StateTuple σs
-
-/-- Run an `SVal` on a tuple of state variables.
-Used like `uncurry f (by assumption)` to implement idiom notation. -/
-def uncurry {σs : List Type} (f : SVal σs σ) (tuple : StateTuple σs) : σ := match σs with
-| [] => f
-| _ :: _ => uncurry (f tuple.1) tuple.2
-
-@[simp]
-theorem uncurry_pure {σs : List Type} {s : σ} {tuple : StateTuple σs} :
-  uncurry (σs:=σs) (pure s) tuple = s := by induction σs <;> simp[uncurry, *]
-
-@[simp]
-theorem uncurry_nil {m : SVal [] α} :
-  uncurry m () = m := rfl
-
-@[simp]
-theorem uncurry_cons {σs : List Type} {s : σ} {m : SVal (σ::σs) α} {tuple : StateTuple σs} :
-  uncurry (σs:=(σ::σs)) m (s, tuple) = uncurry (m s) tuple := rfl
-
-/-- Function used to implement idiom notation.
-```
-example : SVal [Nat, Bool] := idiom fun tpl => SVal.pure (1 + uncurry (getThe Nat) + 3)
-```
- -/
-def idiom {σs : List Type} (f : StateTuple σs → SVal σs α) : SVal σs α := match σs with
-| [] => f ()
-| _ :: _ => fun s => idiom (fun tuple => f (s, tuple) s)
-@[simp] theorem idiom_nil {f : StateTuple [] → SVal [] α} : idiom f = f () := rfl
-@[simp] theorem idiom_cons {σs : List Type} {f : StateTuple (σ::σs) → SVal (σ::σs) α} {s : σ} : idiom f s = idiom (fun tuple => f (s, tuple) s) := rfl
-@[simp] theorem idiom_pure {σs : List Type} {f : SVal σs α} : idiom (fun _ => f) = f := by induction σs <;> simp[idiom, *]
-
 class GetTy (σ : Type) (σs : List Type) where
   get : SVal σs σ
 
@@ -68,3 +32,21 @@ instance [GetTy σ₁ σs] : GetTy σ₁ (σ₂ :: σs) where
 def getThe {σs : List Type} (σ : Type) [GetTy σ σs] : SVal σs σ := GetTy.get
 @[simp] theorem getThe_here {σs : List Type} (σ : Type) (s : σ) : getThe (σs := σ::σs) σ s = pure s := rfl
 @[simp] theorem getThe_there {σs : List Type} [GetTy σ σs] (σ' : Type) (s : σ') : getThe (σs := σ'::σs) σ s = getThe (σs := σs) σ := rfl
+
+def EscapeFun (σs : List Type) := { f : ∀ α, SVal σs α → α // ∀ α (a : α), f α (pure a) = a }
+def EscapeFun.id : EscapeFun [] := ⟨fun _ m => m, fun _ _ => rfl⟩
+def EscapeFun.cons (s : σ) (fn : EscapeFun σs) : EscapeFun (σ::σs) :=
+  ⟨fun α m => fn.1 α (m s), fn.2⟩
+
+def GetTy.applyEscape {σs : List Type} (f : SVal σs σ) (escape : EscapeFun σs) : σ := escape.1 σ f
+@[simp]
+theorem GetTy.applyEscape_pure {σs : List Type} {s : σ} {escape : EscapeFun σs} :
+  GetTy.applyEscape (σs:=σs) (pure s) escape = s := by simp[applyEscape, escape.property]
+
+@[simp]
+theorem GetTy.applyEscape_id {m : SVal [] α} :
+  GetTy.applyEscape m EscapeFun.id = m := rfl
+
+@[simp]
+theorem GetTy.applyEscape_cons {σs : List Type} {s : σ} {m : SVal (σ::σs) α} {escape : EscapeFun σs} :
+  GetTy.applyEscape (σs:=(σ::σs)) m (SVal.EscapeFun.cons s escape) = SVal.GetTy.applyEscape (m s) escape := rfl
